mostly trying stuff out because none of the previous stuff works

theories/input_lang_delim/interp.v
@@ -2,197 +2,195 @@
 From gitrees Require Import gitree.
 From gitrees.input_lang_delim Require Import lang.
 Require Import gitrees.lang_generic_sem.
+From iris.algebra Require Import gmap excl auth gmap_view.
+From iris.proofmode Require Import classes tactics.
+From iris.base_logic Require Import algebra.
+From iris.heap_lang Require Export locations.
 
 Require Import Binding.Lib.
 Require Import Binding.Set.
 
-Notation stateO := (leibnizO state).
 
-Program Definition inputE : opInterp :=
-  {|
-    Ins := unitO;
-    Outs := natO;
-  |}.
-Program Definition outputE : opInterp :=
-  {|
-    Ins := natO;
-    Outs := unitO;
-  |}.
+(** * State *)
 
-Program Definition shiftE : opInterp :=
+Definition stateF : oFunctor := (gmapOF unitO (▶ ∙))%OF.
+
+#[local] Instance state_inhabited : Inhabited (stateF ♯ unitO).
+Proof. apply _. Qed.
+#[local] Instance state_cofe X `{!Cofe X} : Cofe (stateF ♯ X).
+Proof. apply _. Qed.
+
+
+
+(** * Signatures *)
+
+Program Definition readE : opInterp :=  {|
+  Ins := unitO;
+  Outs := (▶ ∙);
+|}.
+
+Program Definition writeE : opInterp :=  {|
+  Ins := (▶ ∙);
+  Outs := unitO;
+|}.
+
+Program Definition callccE : opInterp :=
   {|
     Ins := ((▶ ∙ -n> ▶ ∙) -n> ▶ ∙);
     Outs := (▶ ∙);
   |}.
-
-Program Definition resetE : opInterp :=
+Program Definition throwE : opInterp :=
   {|
-    Ins := (▶ ∙);
-    Outs := (▶ ∙);
+    Ins := (▶ ∙ * (▶ ∙ -n> ▶ ∙));
+    Outs := Empty_setO;
   |}.
 
-Definition ioE := @[inputE; outputE; shiftE; resetE].
 
-Definition reify_input X `{Cofe X} : unitO * stateO * (natO -n> laterO X) →
-                                     option (laterO X * stateO) :=
-  λ '(_, σ, k), let '(n, σ') := (update_input σ : prodO natO stateO) in
-                Some (k n, σ').
-#[export] Instance reify_input_ne X `{Cofe X} :
-  NonExpansive (reify_input X : prodO (prodO unitO stateO)
-                                  (natO -n> laterO X) →
-                                  optionO (prodO (laterO X) stateO)).
+Definition delimE := @[readE; writeE; callccE; throwE].
+
+
+Notation op_read := (inl ()).
+Notation op_write := (inr (inl ())).
+Notation op_callcc := (inr (inr (inl ()))).
+Notation op_throw := (inr (inr (inr (inl ())))).
+
+
+Section reifiers.
+
+  Context {X} `{!Cofe X}.
+  Notation state := (stateF ♯ X).
+
+
+  Definition reify_read : unit * state * (laterO X -n> laterO X) →
+                          option (laterO X * state)
+    := λ '(u,σ,κ), x ← σ !! u;
+  Some (κ x, σ).
+  #[export] Instance reify_read_ne :
+    NonExpansive (reify_read : prodO (prodO unitO state)
+                                 (laterO X -n> laterO X) →
+                               optionO (prodO (laterO X) state)).
+  Proof.
+    intros n[[]][[]][[]]. simpl in *.
+    apply option_mbind_ne; first solve_proper.
+    by rewrite H0.
+  Qed.
+
+  Definition reify_write : (laterO X) * state * (unitO -n> laterO X) →
+                           option (laterO X * state)
+    := λ '(n,s,κ), let s' := <[():=n]>s
+                   in Some (κ (), s').
+  #[export] Instance reify_write_ne :
+    NonExpansive (reify_write : prodO (prodO _ state)
+                                  (unitO -n> laterO X) →
+                                optionO (prodO (laterO X) state)).
+  Proof.
+    intros n [[]] [[]] [[]]; simpl in *. solve_proper.
+  Qed.
+
+
+  Definition reify_callcc : ((laterO X -n> laterO X) -n> laterO X) *
+                              state * (laterO X -n> laterO X) →
+                            option (laterO X * state) :=
+    λ '(f, σ, k), Some ((k (f k): laterO X), σ : state).
+  #[export] Instance reify_callcc_ne :
+    NonExpansive (reify_callcc :
+      prodO (prodO ((laterO X -n> laterO X) -n> laterO X) state)
+        (laterO X -n> laterO X) →
+      optionO (prodO (laterO X) state)).
+  Proof. intros ?[[]][[]][[]]. simpl in *. repeat f_equiv; auto. Qed.
+
+
+  Definition reify_throw :
+    ((laterO X * (laterO X -n> laterO X)) * state * (Empty_setO -n> laterO X)) →
+    option (laterO X * state) :=
+    λ '((e, k'), σ, _),
+      Some ((k' e : laterO X), σ : state).
+  #[export] Instance reify_throw_ne :
+    NonExpansive (reify_throw :
+        prodO (prodO (prodO (laterO X) (laterO X -n> laterO X)) state)
+          (Empty_setO -n> laterO X) →
+        optionO (prodO (laterO X) (state))).
+  Proof.
+    intros ?[[[]]][[[]]]?. rewrite /reify_throw.
+    repeat f_equiv; apply H.
+  Qed.
+
+End reifiers.
+
+Canonical Structure reify_delim : sReifier.
 Proof.
-  intros n [[? σ1] k1] [[? σ2] k2]. simpl.
-  intros [[_ ->] Hk]. simpl in *.
-  repeat f_equiv. assumption.
-Qed.
-
-Definition reify_output X `{Cofe X} : (natO * stateO * (unitO -n> laterO X)) →
-                                      optionO (prodO (laterO X) stateO) :=
-  λ '(n, σ, k), Some (k (), ((update_output n σ) : stateO)).
-#[export] Instance reify_output_ne X `{Cofe X} :
-  NonExpansive (reify_output X : prodO (prodO natO stateO)
-                                   (unitO -n> laterO X) →
-                                 optionO (prodO (laterO X) stateO)).
-Proof.
-  intros ? [[]] [[]] []; simpl in *.
-  repeat f_equiv; first assumption; apply H0.
-Qed.
-
-Definition reify_shift X `{Cofe X} : ((laterO X -n> laterO X) -n> laterO X) *
-                                        stateO * (laterO X -n> laterO X) →
-                                      option (laterO X * stateO) :=
-  λ '(f, σ, k), Some ((f k): laterO X, σ : stateO).
-#[export] Instance reify_shift_ne X `{Cofe X} :
-  NonExpansive (reify_shift X :
-    prodO (prodO ((laterO X -n> laterO X) -n> laterO X) stateO)
-      (laterO X -n> laterO X) →
-    optionO (prodO (laterO X) stateO)).
-Proof. intros ?[[]][[]][[]]. simpl in *. repeat f_equiv; auto. Qed.
-
-
-(* CHECK *)
-Definition reify_reset X `{Cofe X} :
-  (laterO X * stateO * (laterO X -n> laterO X)) →
-  option (laterO X * stateO) :=
-  λ '(e, σ, k), Some (k e, σ).
-(* and add the [get_val] in interp. BUT: doesn't it defeat the whole purpose of
-   having reset as an effect? *)
-#[export] Instance reify_reset_ne X `{Cofe X} :
-  NonExpansive (reify_reset X :
-      prodO (prodO (laterO X) stateO) (laterO X -n> laterO X) →
-      optionO (prodO (laterO X) stateO)).
-Proof. intros ?[[]][[]][[]]. simpl in *. by repeat f_equiv. Qed.
-
-
-(* Context {E : opsInterp} {A} `{!Cofe A}. *)
-(* Context {subEff0 : subEff ioE E}. *)
-(* Context {subOfe0 : SubOfe natO A}. *)
-(* Notation IT := (IT E A). *)
-(* Notation ITV := (ITV E A). *)
-
-(* Definition reify_reset : (laterO IT * stateO * (laterO IT -n> laterO IT)) → *)
-(*                          option (laterO IT * stateO) := *)
-(*   λ '(e, σ, k), Some (k $ laterO_map (get_val idfun) e, σ). *)
-(* #[export] Instance reify_reset_ne : *)
-(*   NonExpansive (reify_reset : *)
-(*       prodO (prodO (laterO IT) stateO) (laterO IT -n> laterO IT) → *)
-(*       optionO (prodO (laterO IT) stateO)). *)
-(* Proof. intros ?[[]][[]][[]]. simpl in *. repeat f_equiv; done. Qed. *)
-
-
-
-Canonical Structure reify_io : sReifier.
-Proof.
-  simple refine {| sReifier_ops := ioE;
-                   sReifier_state := stateO
-                |}.
+  simple refine {|
+             sReifier_ops := delimE;
+             sReifier_state := stateF
+           |}.
   intros X HX op.
   destruct op as [ | [ | [ | [| []]]]]; simpl.
-  - simple refine (OfeMor (reify_input X)).
-  - simple refine (OfeMor (reify_output X)).
-  - simple refine (OfeMor (reify_shift X)).
-  - simple refine (OfeMor (reify_reset X)).
+  - simple refine (OfeMor (reify_read)).
+  - simple refine (OfeMor (reify_write)).
+  - simple refine (OfeMor (reify_callcc)).
+  - simple refine (OfeMor (reify_throw)).
 Defined.
 
 
-Notation op_input := (inl ()).
-Notation op_output := (inr (inl ())).
-Notation op_shift := (inr (inr (inl ()))).
-Notation op_reset := (inr (inr (inr (inl ())))).
 
 Section constructors.
   Context {E : opsInterp} {A} `{!Cofe A}.
-  Context {subEff0 : subEff ioE E}.
+  Context {subEff0 : subEff delimE E}.
   Context {subOfe0 : SubOfe natO A}.
+  Context {subOfe1 : SubOfe unitO A}.
   Notation IT := (IT E A).
   Notation ITV := (ITV E A).
 
-  Program Definition INPUT : (nat -n> IT) -n> IT :=
-    λne k, Vis (E:=E) (subEff_opid op_input)
-             (subEff_ins (F:=ioE) (op:=op_input) ())
-             (NextO ◎ k ◎ (subEff_outs (F:=ioE) (op:=op_input))^-1).
+
+  Program Definition READ : IT :=
+    Vis (E:=E) (subEff_opid $ op_read)
+      (subEff_ins (F:=delimE) (op:=op_read) ())
+      ((subEff_outs (F:=delimE) (op:=op_read))^-1).
+
+
+  Program Definition WRITE :  IT -n> IT :=
+    λne a, Vis (E:=E) (subEff_opid $ op_write)
+                (subEff_ins (F:=delimE) (op:=op_write) (Next a))
+                (λne _, Next (Ret ())).
   Solve Obligations with solve_proper.
 
-  Program Definition OUTPUT_ : nat -n> IT -n> IT :=
-    λne m α, Vis (E:=E) (subEff_opid op_output)
-                        (subEff_ins (F:=ioE) (op:=op_output) m)
-                        (λne _, NextO α).
-  Solve All Obligations with solve_proper_please.
-  Program Definition OUTPUT : nat -n> IT := λne m, OUTPUT_ m (Ret 0).
 
-
-  Program Definition SHIFT_ : ((laterO IT -n> laterO IT) -n> laterO IT) -n>
+  Program Definition CALLCC_ : ((laterO IT -n> laterO IT) -n> laterO IT) -n>
                                 (laterO IT -n> laterO IT) -n>
                                 IT :=
-    λne f k, Vis (E:=E) (subEff_opid op_shift)
-             (subEff_ins (F:=ioE) (op:=op_shift) f)
-             (k ◎ (subEff_outs (F:=ioE) (op:=op_shift))^-1).
+    λne f k, Vis (E:=E) (subEff_opid op_callcc)
+             (subEff_ins (F:=delimE) (op:=op_callcc) f)
+             (k ◎ (subEff_outs (F:=delimE) (op:=op_callcc))^-1).
   Solve All Obligations with solve_proper.
 
-  Program Definition SHIFT : ((laterO IT -n> laterO IT) -n> laterO IT) -n> IT :=
-    λne f, SHIFT_ f (idfun).
+  Program Definition CALLCC : ((laterO IT -n> laterO IT) -n> laterO IT) -n> IT :=
+    λne f, CALLCC_ f (idfun).
   Solve Obligations with solve_proper.
 
-  (* Program Definition RESET : laterO IT -n> IT := *)
-  (*   λne e, Vis (E:=E) (subEff_opid op_reset) *)
-  (*              (subEff_ins (F := ioE) (op := op_reset) e) *)
-  (*              (subEff_outs (F := ioE) (op := op_reset)^-1). *)
-  (* Solve All Obligations with solve_proper. *)
-
-  Program Definition RESET_ : (laterO IT -n> laterO IT) -n>
-                                laterO IT -n>
-                                IT :=
-      λne k e, Vis (E:=E) (subEff_opid op_reset)
-                 (subEff_ins (F := ioE) (op := op_reset) e)
-                 (k ◎ subEff_outs (F := ioE) (op := op_reset)^-1).
-  Solve Obligations with solve_proper.
-
-  Program Definition RESET : laterO IT -n> IT :=
-    RESET_ idfun.
-
-
-  Lemma hom_INPUT k f `{!IT_hom f} : f (INPUT k) ≡ INPUT (OfeMor f ◎ k).
+  Lemma hom_CALLCC_ k e f `{!IT_hom f} :
+    f (CALLCC_ e k) ≡ CALLCC_ e (laterO_map (OfeMor f) ◎ k).
   Proof.
-    unfold INPUT.
-    rewrite hom_vis/=. repeat f_equiv.
-    intro x. cbn-[laterO_map]. rewrite laterO_map_Next.
-    done.
-  Qed.
-  Lemma hom_OUTPUT_ m α f `{!IT_hom f} : f (OUTPUT_ m α) ≡ OUTPUT_ m (f α).
-  Proof.
-    unfold OUTPUT.
-    rewrite hom_vis/=. repeat f_equiv.
-    intro x. cbn-[laterO_map]. rewrite laterO_map_Next.
-    done.
-  Qed.
-
-  Lemma hom_SHIFT_ k e f `{!IT_hom f} :
-    f (SHIFT_ e k) ≡ SHIFT_ e (laterO_map (OfeMor f) ◎ k).
-  Proof.
-    unfold SHIFT_.
+    unfold CALLCC_.
     rewrite hom_vis/=.
     f_equiv. by intro.
+  Qed.
+
+  Program Definition THROW : IT -n> (laterO IT -n> laterO IT) -n> IT :=
+    λne e k, Vis (E:=E) (subEff_opid op_throw)
+               (subEff_ins (F:=delimE) (op:=op_throw)
+                  (NextO e, k))
+               (λne x, Empty_setO_rec _ ((subEff_outs (F:=delimE) (op:=op_throw))^-1 x)).
+  Next Obligation.
+    solve_proper_prepare.
+    destruct ((subEff_outs ^-1) x).
+  Qed.
+  Next Obligation.
+    intros; intros ???; simpl.
+    repeat f_equiv. assumption.
+  Qed.
+  Next Obligation.
+    intros ?????; simpl.
+    repeat f_equiv; assumption.
   Qed.
 
 
@@ -201,114 +199,263 @@ End constructors.
 Section weakestpre.
   Context {sz : nat}.
   Variable (rs : gReifiers sz).
-  Context {subR : subReifier reify_io rs}.
+  Context {subR : subReifier reify_delim rs}.
   Notation F := (gReifiers_ops rs).
   Context {R} `{!Cofe R}.
   Context `{!SubOfe natO R}.
+  Context `{!SubOfe unitO R}.
   Notation IT := (IT F R).
   Notation ITV := (ITV F R).
-  Context `{!invGS Σ, !stateG rs R Σ}.
+  Notation state := (stateF ♯ IT).
+
+
+  (* a separate ghost state for keeping track of locations *)
+  Definition istate := gmap_viewUR unit (laterO IT).
+  Class heapPreG Σ := HeapPreG { heapPreG_inG :: inG Σ istate }.
+  Class heapG Σ := HeapG {
+      heapG_inG :: inG Σ istate;
+      heapG_name : gname;
+    }.
+  Definition heapΣ : gFunctors := GFunctor istate.
+  #[export] Instance subG_heapΣ {Σ} : subG heapΣ Σ → heapPreG Σ.
+  Proof. solve_inG. Qed.
+
+  Lemma new_heapG σ `{!heapPreG Σ} :
+    (⊢ |==> ∃ `{!heapG Σ}, own heapG_name (●V σ): iProp Σ)%I.
+  Proof.
+    iMod (own_alloc (●V σ)) as (γ) "H".
+    { apply gmap_view_auth_valid. }
+    pose (sg := {| heapG_inG := _; heapG_name := γ |}).
+    iModIntro. iExists sg. by iFrame.
+  Qed.
+
+  Context `{!invGS_gen HasLc Σ, !stateG rs R Σ}.
   Notation iProp := (iProp Σ).
 
-  Lemma wp_input' (σ σ' : stateO) (n : nat) (k : natO -n> IT) (κ : IT -n> IT)
-    `{!IT_hom κ} Φ s :
-    update_input σ = (n, σ') ->
-    has_substate σ -∗
-    ▷ (£ 1 -∗ has_substate σ' -∗ WP@{rs} (κ ◎ k $ n) @ s {{ Φ }}) -∗
-    WP@{rs} κ (INPUT k) @ s {{ Φ }}.
+  (** * The ghost state theory for the heap *)
+
+  Context `{!heapG Σ}.
+
+  Definition heap_ctx := inv (nroot.@"storeE")
+                        (∃ σ, £ 1 ∗ has_substate σ ∗ own heapG_name (●V σ))%I.
+
+  Definition pointsto (u : unit) (α : IT) : iProp :=
+    own heapG_name $ gmap_view_frag u (DfracOwn 1) (Next α).
+
+
+
+  Lemma istate_alloc α u σ :
+    σ !! u = None →
+    own heapG_name (●V σ) ==∗ own heapG_name (●V (<[u:=(Next α)]>σ))
+                   ∗ pointsto u α.
   Proof.
-    iIntros (Hσ) "Hs Ha".
-    rewrite hom_INPUT. simpl.
-    iApply (wp_subreify with "Hs").
-    + simpl. by rewrite Hσ.
-    + by rewrite ofe_iso_21.
-    + done.
+    iIntros (Hl) "H".
+    iMod (own_update with "H") as "[$ $]".
+    { apply (gmap_view_alloc _ u (DfracOwn 1) (Next α)); eauto.
+      done. }
+    done.
+  Qed.
+  Lemma istate_read u α σ :
+    own heapG_name (●V σ) -∗ pointsto u α -∗ σ !! u ≡ Some (Next α).
+  Proof.
+    iIntros "Ha Hf".
+    iPoseProof (own_valid_2 with "Ha Hf") as "H".
+    rewrite gmap_view_both_validI.
+    iDestruct "H" as "[_ Hval]". done.
+  Qed.
+  Lemma istate_loc_dom u α σ :
+    own heapG_name (●V σ) -∗ pointsto u α -∗ ⌜is_Some (σ !! u)⌝.
+  Proof.
+    iIntros "Hinv Hloc".
+    iPoseProof (istate_read with "Hinv Hloc") as "Hl".
+    destruct (σ !! u) ; eauto.
+    by rewrite option_equivI.
+  Qed.
+  Lemma istate_write u α β σ :
+    own heapG_name (●V σ) -∗ pointsto u α ==∗ own heapG_name (●V <[u:=(Next β)]>σ)
+                                  ∗ pointsto u β.
+  Proof.
+    iIntros "H Hu".
+    iMod (own_update_2 with "H Hu") as "[$ $]".
+    { apply (gmap_view_update). }
+    done.
+  Qed.
+  Lemma istate_delete u α σ :
+    own heapG_name (●V σ) -∗ pointsto u α ==∗ own heapG_name (●V delete u σ).
+  Proof.
+    iIntros "H Hu".
+    iMod (own_update_2 with "H Hu") as "$".
+    { apply (gmap_view_delete). }
+    done.
   Qed.
 
-  Lemma wp_input (σ σ' : stateO) (n : nat) (k : natO -n> IT) Φ s :
-    update_input σ = (n, σ') →
-    has_substate σ -∗
-    ▷ (£ 1 -∗ has_substate σ' -∗ WP@{rs} (k n) @ s {{ Φ }}) -∗
-    WP@{rs} (INPUT k) @ s {{ Φ }}.
+
+  (** * The symbolic execution rules *)
+
+  (** ** READ *)
+
+  Lemma wp_read_atomic (l : unit)  E1 E2 s Φ
+    (k : IT -n> IT) `{!IT_hom k} :
+    nclose (nroot.@"storeE") ## E1 →
+    heap_ctx -∗
+    (|={E1,E2}=> ∃ α, ▷ pointsto l α ∗
+        ▷ ▷ (pointsto l α ={E2,E1}=∗ WP@{rs} k α @ s {{ Φ }})) -∗
+    WP@{rs} k READ @ s {{ Φ }}.
   Proof.
-    eapply (wp_input' σ σ' n k idfun).
+    iIntros (Hee) "#Hcxt H". rewrite hom_vis. simpl.
+    match goal with
+    | |- context G [Vis ?a ?b ?c] => assert (c ≡ laterO_map k ◎ subEff_outs (op:=op_read) ^-1) as ->
+    end; first solve_proper.
+    iApply wp_subreify'.
+    iInv (nroot.@"storeE") as (σ) "[>Hlc [Hs Hh]]" "Hcl".
+    iApply (fupd_mask_weaken E1).
+    { set_solver. }
+    iIntros "Hwk".
+    iMod "H" as (α) "[Hp Hback]".
+    iApply (lc_fupd_elim_later with "Hlc").
+    iNext.
+    iAssert (⌜is_Some (σ !! l)⌝)%I as "%Hdom".
+    { iApply (istate_loc_dom with "Hh Hp"). }
+    destruct Hdom as [x Hx].
+    destruct (Next_uninj x) as [β' Hb'].
+    iAssert ((σ !! l ≡ Some (Next α)))%I as "#Hlookup".
+    { iApply (istate_read with "Hh Hp"). }
+    iAssert (▷ (β' ≡ α))%I as "#Hba".
+    { rewrite Hx. rewrite option_equivI.
+      rewrite Hb'. by iNext. }
+    iClear "Hlookup".
+    iExists σ,(Next $ k β'),σ,(k β').
+    iFrame "Hs".
+    repeat iSplit.
+    - assert ((option_bind _ _ (λ x, Some (laterO_map k x, σ)) (σ !! l)) ≡
+                 (option_bind _ _ (λ x, Some (x, σ)) (Some (Next $ k β')))) as H.
+      { rewrite Hx. simpl. rewrite Hb'. by rewrite later_map_Next. }
+      simpl in H.
+      rewrite <-H.
+      unfold mbind.
+      simpl.
+      iPureIntro.
+      f_equiv; last done.
+      intros ???.
+      do 2 f_equiv. rewrite H0.
+      by rewrite ofe_iso_21.
+    - done.
+    - iNext. iIntros "Hlc Hs".
+      iMod ("Hback" with "Hp") as "Hback".
+      iMod "Hwk" .
+      iMod ("Hcl" with "[Hlc Hh Hs]") as "_".
+      { iExists _. by iFrame. }
+      iRewrite "Hba". done.
   Qed.
 
-  (* Lemma wp_input (σ σ' : stateO) (n : nat) (k : natO -n> IT) Φ s : *)
-  (*   update_input σ = (n, σ') → *)
-  (*   has_substate σ -∗ *)
-  (*   ▷ (£ 1 -∗ has_substate σ' -∗ WP@{rs} (k n) @ s {{ Φ }}) -∗ *)
-  (*   WP@{rs} (INPUT k) @ s {{ Φ }}. *)
-  (* Proof. *)
-  (*   intros Hs. iIntros "Hs Ha". *)
-  (*   unfold INPUT. simpl. *)
-  (*   iApply (wp_subreify with "Hs"). *)
-  (*   { simpl. by rewrite Hs. } *)
-  (*   { simpl. by rewrite ofe_iso_21. } *)
-  (*   iModIntro. done. *)
-  (* Qed. *)
-
-  Lemma wp_output' (σ σ' : stateO) (n : nat) (κ : IT -n> IT)
-    `{!IT_hom κ} Φ s :
-    update_output n σ = σ' →
-    has_substate σ -∗
-    ▷ (£ 1 -∗ has_substate σ' -∗ WP@{rs} (κ (Ret 0)) @ s {{ Φ }}) -∗
-    WP@{rs} κ (OUTPUT n) @ s {{ Φ }}.
+  Lemma wp_read (l : unit) (α : IT) s Φ
+    (k : IT -n> IT) `{!IT_hom k} :
+    heap_ctx -∗
+    ▷ pointsto l α -∗
+    ▷ ▷ (pointsto l α -∗ WP@{rs} k α @ s {{ Φ }}) -∗
+    WP@{rs} k READ @ s {{ Φ }}.
   Proof.
-    iIntros (Hσ) "Hs Ha".
-    rewrite /OUTPUT hom_OUTPUT_.
-    iApply (wp_subreify with "Hs").
-    + simpl. by rewrite Hσ.
-    + done.
-    + done.
+    iIntros "#Hcxt Hp Ha".
+    iApply (wp_read_atomic _ (⊤∖ nclose (nroot.@"storeE")) with "[$]").
+    { set_solver. }
+    iModIntro. iExists _; iFrame.
+    iNext. iNext. iIntros "Hl".
+    iModIntro. by iApply "Ha".
+  Qed.
+
+  (** ** WRITE *)
+
+  Lemma wp_write_atomic  E1 E2 β s Φ
+    (k : IT -n> IT) `{!IT_hom k} :
+    nclose (nroot.@"storeE") ## E1 →
+    heap_ctx -∗
+    (|={E1,E2}=> ∃ α, ▷ pointsto () α ∗
+        ▷ ▷ (pointsto () β ={E2,E1}=∗ WP@{rs} k (Ret ()) @ s {{ Φ }})) -∗
+    WP@{rs} k (WRITE β) @ s {{ Φ }}.
+  Proof.
+    iIntros (Hee) "#Hcxt H". rewrite hom_vis. simpl.
+    iApply wp_subreify'.
+    iInv (nroot.@"storeE") as (σ) "[>Hlc [Hs Hh]]" "Hcl".
+    iApply (fupd_mask_weaken E1).
+    { set_solver. }
+    iIntros "Hwk".
+    iMod "H" as (α) "[Hp Hback]".
+    iAssert (▷ ⌜is_Some (σ !! tt)⌝)%I as "#Hdom".
+    { iNext. iApply (istate_loc_dom with "Hh Hp"). }
+    iDestruct "Hdom" as ">%Hdom".
+    destruct Hdom as [x Hx].
+    destruct (Next_uninj x) as [α' Ha'].
+    iApply (lc_fupd_elim_later with "Hlc").
+    iNext.
+    iExists σ, (Next $ k (Ret ())), (<[():=Next β]>σ), (k $ Ret ()).
+    iFrame "Hs".
+    iSimpl. repeat iSplit; [ by rewrite later_map_Next | done | ].
+    iNext. iIntros "Hlc".
+    iMod (istate_write _ _ β with "Hh Hp") as "[Hh Hp]".
+    iIntros "Hs".
+    iMod ("Hback" with "Hp") as "Hback".
+    iMod "Hwk" .
+    iMod ("Hcl" with "[Hlc Hh Hs]") as "_".
+    { iExists _. iFrame. }
+    done.
+  Qed.
+
+  Lemma wp_write (α β : IT) s Φ (k : IT -n> IT) `{!IT_hom k} :
+    heap_ctx -∗
+    ▷ pointsto () α -∗
+    ▷▷ (pointsto () β -∗ WP@{rs} k (Ret ()) @ s {{ Φ }}) -∗
+    WP@{rs} k $ WRITE β @ s {{ Φ }}.
+  Proof.
+    iIntros "#Hctx Hp Ha".
+    iApply (wp_write_atomic (⊤∖ nclose (nroot.@"storeE")) with "[$]").
+    { set_solver. }
+    iModIntro. iExists _; iFrame.
+    iNext. iNext. iIntros "Hl".
+    iModIntro. by iApply "Ha".
   Qed.
 
 
-  Lemma wp_output (σ σ' : stateO) (n : nat) Φ s :
-    update_output n σ = σ' →
+  (** ** THROW *)
+
+  Lemma wp_throw' (σ : state) (f : laterO IT -n> laterO IT) (x : IT)
+    (κ : IT -n> IT) `{!IT_hom κ} Φ s :
     has_substate σ -∗
-    ▷ (£ 1 -∗ has_substate σ' -∗ Φ (RetV 0)) -∗
-    WP@{rs} (OUTPUT n) @ s {{ Φ }}.
+    ▷ (£ 1 -∗ has_substate σ -∗ WP@{rs} later_car $ f (Next x) @ s {{ Φ }}) -∗
+    WP@{rs} κ (THROW x f) @ s {{ Φ }}.
   Proof.
-    iIntros (Hσ) "Hs Ha".
-    iApply (wp_output' _ _ _ idfun with "Hs [Ha]"); first done.
-    simpl. iNext. iIntros "Hcl Hs".
-    iApply wp_val. iApply ("Ha" with "Hcl Hs").
+    iIntros "Hs Ha". rewrite /THROW. simpl.
+    rewrite hom_vis.
+    destruct (Next_uninj (f (Next x))) as [α Hα].
+    iApply (wp_subreify with "Hs"); simpl.
+    + reflexivity.
+    + apply Hα.
+    + by assert (α ≡ later_car (f (Next x))) as -> by done.
   Qed.
 
-  (* Lemma wp_throw' (σ : stateO) (f : laterO (IT -n> IT)) (x : IT) *)
-  (*   (κ : IT -n> IT) `{!IT_hom κ} Φ s : *)
-  (*   has_substate σ -∗ *)
-  (*   ▷ (£ 1 -∗ has_substate σ -∗ WP@{rs} (later_car f) x @ s {{ Φ }}) -∗ *)
-  (*   WP@{rs} κ (THROW x f) @ s {{ Φ }}. *)
-  (* Proof. *)
-  (*   iIntros "Hs Ha". rewrite /THROW. simpl. *)
-  (*   rewrite hom_vis. *)
-  (*   iApply (wp_subreify with "Hs"); simpl; done. *)
-  (* Qed. *)
+  Lemma wp_throw (σ : state) (f : laterO IT -n> laterO IT) (x : IT) Φ s :
+    has_substate σ -∗
+    ▷ (£ 1 -∗ has_substate σ -∗ WP@{rs} later_car $ f $ Next x @ s {{ Φ }}) -∗
+    WP@{rs} (THROW x f) @ s {{ Φ }}.
+  Proof.
+    iApply (wp_throw' _ _ _ idfun).
+  Qed.
 
-  (* Lemma wp_throw (σ : stateO) (f : laterO (IT -n> IT)) (x : IT) Φ s : *)
-  (*   has_substate σ -∗ *)
-  (*   ▷ (£ 1 -∗ has_substate σ -∗ WP@{rs} later_car f x @ s {{ Φ }}) -∗ *)
-  (*   WP@{rs} (THROW x f) @ s {{ Φ }}. *)
-  (* Proof. *)
-  (*   iApply (wp_throw' _ _ _ idfun). *)
-  (* Qed. *)
+  (** ** CALL/CC *)
 
-  Lemma wp_shift (σ : stateO) (f : (laterO IT -n> laterO IT) -n> laterO IT)
+  Lemma wp_callcc (σ : state) (f : (laterO IT -n> laterO IT) -n> laterO IT)
     (k : IT -n> IT) {Hk : IT_hom k} Φ s :
     has_substate σ -∗
-    ▷ (£ 1 -∗ has_substate σ -∗ WP@{rs} idfun (later_car (f (laterO_map k))) @ s {{ Φ }}) -∗
-    WP@{rs} (k (SHIFT f)) @ s {{ Φ }}.
+    ▷ (£ 1 -∗ has_substate σ -∗ WP@{rs} k (later_car (f (laterO_map k))) @ s {{ Φ }}) -∗
+    WP@{rs} (k (CALLCC f)) @ s {{ Φ }}.
   Proof.
     iIntros "Hs Ha".
-    unfold SHIFT. simpl.
+    unfold CALLCC. simpl.
     rewrite hom_vis.
-    iApply (wp_subreify _ _ _ _ _ _ _ ((later_map idfun ((f (laterO_map k))))) with "Hs").
+    iApply (wp_subreify _ _ _ _ _ _ _ ((later_map k ((f (laterO_map k))))) with "Hs").
     {
       simpl.
       repeat f_equiv.
-      - rewrite ccompose_id_l later_map_id.
+      - rewrite ofe_iso_21.
         f_equiv. intro x. simpl.
         by rewrite ofe_iso_21.
       - reflexivity.
@@ -323,12 +470,14 @@ End weakestpre.
 Section interp.
   Context {sz : nat}.
   Variable (rs : gReifiers sz).
-  Context {subR : subReifier reify_io rs}.
+  Context {subR : subReifier reify_delim rs}.
   Context {R} `{CR : !Cofe R}.
   Context `{!SubOfe natO R}.
+  Context `{!SubOfe unitO R}.
   Notation F := (gReifiers_ops rs).
   Notation IT := (IT F R).
   Notation ITV := (ITV F R).
+  Notation state := (stateF ♯ IT).
   Context `{!invGS Σ, !stateG rs R Σ}.
   Notation iProp := (iProp Σ).
 
@@ -338,82 +487,55 @@ Section interp.
     solve_proper.
   Qed.
 
-  (** Interpreting individual operators *)
-  Program Definition interp_input {A} : A -n> IT :=
-    λne env, INPUT Ret.
-  Program Definition interp_output {A} (t : A -n> IT) : A -n> IT :=
-    get_ret OUTPUT ◎ t.
-  Local Instance interp_ouput_ne {A} : NonExpansive2 (@interp_output A).
-  Proof. solve_proper. Qed.
+  (** * Interpreting individual operators *)
 
-  (* Program Definition interp_shift {S} *)
-  (*   (e : @interp_scope F R _ (inc S) -n> IT) : interp_scope S -n> IT := *)
-  (*   λne env, SHIFT (λne (k : laterO IT -n> laterO IT), *)
-  (*                      (Next (e (@extend_scope F R _ _ env *)
-  (*                                  (Fun (Next (λne x, Tau (k (Next x))))))))). *)
-  (* Next Obligation. *)
-  (*   solve_proper. *)
-  (* Qed. *)
-  (* Next Obligation. *)
-  (*   solve_proper_prepare. *)
-  (*   repeat f_equiv. *)
-  (*   intros [| a]; simpl; last solve_proper. *)
-  (*   repeat f_equiv. *)
-  (*   intros ?; simpl. *)
-  (*   by repeat f_equiv. *)
-  (* Qed. *)
-  (* Next Obligation. *)
-  (*   solve_proper_prepare. *)
-  (*   repeat f_equiv. *)
-  (*   intros ?; simpl. *)
-  (*   repeat f_equiv. *)
-  (*   intros [| a]; simpl; last solve_proper. *)
-  (*   repeat f_equiv. *)
-  (* Qed. *)
-
-  Program Definition interp_shift {S} (e : S -n> IT) : S -n> IT :=
-    λne env, get_fun (λne (f : laterO (IT -n> IT)),
-                        SHIFT (λne (k : laterO IT -n> laterO IT),
-                                  laterO_ap f (Next (λit x, Tau (k (Next x)))))) (e env).
+  (** ** RESET *)
+  Program Definition interp_reset (e : IT) : IT :=
+    get_val (λne v,
+    CALLCC (λne (k : laterO IT -n> laterO IT),
+              Next $
+              LET READ (λne m, SEQ
+                                 (WRITE (λit r, SEQ (WRITE m) (THROW r k)))
+                                 (APP' READ v)))) e.
   Solve Obligations with solve_proper.
   Next Obligation.
-    solve_proper_prepare. repeat f_equiv. intro. simpl. by repeat f_equiv.
+    intros e v k n ???. repeat f_equiv. intro. simpl. solve_proper.
   Qed.
   Next Obligation.
-    Opaque laterO_ap.
-    solve_proper_prepare. repeat f_equiv. intro. simpl.
-    by apply later_ap_ne.
-    Transparent laterO_ap.
+    intros e v n ???. repeat f_equiv. by do 2 (intro; simpl; repeat f_equiv).
   Qed.
   Next Obligation.
-    solve_proper_prepare. by repeat f_equiv.
+    intros e n ???. f_equiv. intro. simpl. solve_proper_please.
   Qed.
 
-  Program Definition interp_reset {S} (e : S -n> IT) : S -n> IT :=
-    λne env, get_val idfun (RESET (Next (e env))).
-  Solve All Obligations with solve_proper_please.
+  #[export] Instance interp_reset_ne :
+    NonExpansive (interp_reset).
+  Proof.
+    solve_proper.
+    (* intros n ???. rewrite /interp_reset. simpl. repeat f_equiv. done. *)
+    (* by do 2 (intro; simpl; repeat f_equiv). *)
+  Qed.
 
-  (* Program Definition interp_throw {A} (e : A -n> IT) (k : A -n> IT) *)
-  (*   : A -n> IT := *)
-  (*   λne env, get_val (λne x, get_fun (λne (f : laterO (IT -n> IT)), *)
-  (*                                THROW x f) (k env)) (e env). *)
-  (* Next Obligation. *)
-  (*   solve_proper. *)
-  (* Qed. *)
-  (* Next Obligation. *)
-  (*   solve_proper_prepare. *)
-  (*   repeat f_equiv. *)
-  (*   intro; simpl. *)
-  (*   by repeat f_equiv. *)
-  (* Qed. *)
-  (* Next Obligation. *)
-  (*   solve_proper_prepare. *)
-  (*   repeat f_equiv; last done. *)
-  (*   intro; simpl. *)
-  (*   by repeat f_equiv. *)
-  (* Qed. *)
+  (** ** SHIFT *)
+  Program Definition interp_shift {S} (e : S -n> IT) : S -n> IT :=
+    λne env, CALLCC (λne (k : laterO IT -n> laterO IT),
+                       Next (APP'
+                               READ
+                               (APP'
+                                  (e env)
+                                  (λit x, interp_reset (THROW x k))))).
+  Next Obligation.
+    intros S e env k n ???. by repeat f_equiv.
+  Qed.
+  Next Obligation.
+    intros S e env n ???. repeat f_equiv. intro. simpl. by repeat f_equiv.
+  Qed.
+  Next Obligation.
+    intros S e n ???. f_equiv. by intro; simpl; repeat f_equiv.
+  Qed.
 
 
+  (** ** NATOP *)
   Program Definition interp_natop {A} (op : nat_op) (t1 t2 : A -n> IT) : A -n> IT :=
     λne env, NATOP (do_natop op) (t1 env) (t2 env).
   Solve All Obligations with solve_proper_please.
@@ -422,6 +544,8 @@ Section interp.
   Proof. solve_proper. Qed.
   Typeclasses Opaque interp_natop.
 
+
+  (** ** REC *)
   Opaque laterO_map.
   Program Definition interp_rec_pre {S : Set} (body : @interp_scope F R _ (inc (inc S)) -n> IT)
     : laterO (@interp_scope F R _ S -n> IT) -n> @interp_scope F R _ S -n> IT :=
@@ -474,6 +598,8 @@ Section interp.
     simpl. unfold ir_unf. intro. simpl. reflexivity.
   Qed.
 
+
+  (** ** APP *)
   Program Definition interp_app {A} (t1 t2 : A -n> IT) : A -n> IT :=
     λne env, APP' (t1 env) (t2 env).
   Solve All Obligations with first [ solve_proper | solve_proper_please ].
@@ -481,6 +607,7 @@ Section interp.
   Proof. solve_proper. Qed.
   Typeclasses Opaque interp_app.
 
+  (** ** IF *)
   Program Definition interp_if {A} (t0 t1 t2 : A -n> IT) : A -n> IT :=
     λne env, IF (t0 env) (t1 env) (t2 env).
   Solve All Obligations with first [ solve_proper | solve_proper_please ].
@@ -488,9 +615,11 @@ Section interp.
     Proper ((dist n) ==> (dist n) ==> (dist n) ==> (dist n)) (@interp_if A).
   Proof. solve_proper. Qed.
 
+  (** ** NAT *)
   Program Definition interp_nat (n : nat) {A} : A -n> IT :=
     λne env, Ret n.
 
+  (** ** CONT *)
   Program Definition interp_cont {S} (e : @interp_scope F R _ (inc S) -n> IT) :
     interp_scope S -n> IT :=
     λne env, (Fun (Next (λne x, Tick $ e (@extend_scope F R _ _ env x)))).
@@ -505,40 +634,9 @@ Section interp.
     intros [|z]; eauto.
   Qed.
 
-  (*   (e : @interp_scope F R _ (inc S) -n> IT) : interp_scope S -n> IT := *)
-  (*   λne env, SHIFT (λne (k : laterO IT -n> laterO IT), *)
-  (*                      (Next (e (@extend_scope F R _ _ env *)
-  (*                                  (Fun (Next (λne x, Tau (k (Next x))))))))). *)
-
-
-
-  (* Program Definition interp_natoprk {A} (op : nat_op) *)
-  (*   (q : A -n> IT) *)
-  (*   (K : A -n> (IT -n> IT)) : A -n> (IT -n> IT) := *)
-  (*   λne env t, interp_natop op q (λne env, K env t) env. *)
-  (* Solve All Obligations with solve_proper. *)
-
-  (* Program Definition interp_natoplk {A} (op : nat_op) *)
-  (*   (K : A -n> (IT -n> IT)) *)
-  (*   (q : A -n> IT) : A -n> (IT -n> IT) := *)
-  (*   λne env t, interp_natop op (λne env, K env t) q env. *)
-  (* Solve All Obligations with solve_proper. *)
-
-  (* Program Definition interp_ifk {A} (K : A -n> (IT -n> IT)) (q : A -n> IT) *)
-  (*   (p : A -n> IT) : A -n> (IT -n> IT) := *)
-  (*   λne env t, interp_if (λne env, K env t) q p env. *)
-  (* Solve All Obligations with solve_proper. *)
-
-
-  (* Program Definition interp_throwlk {A} (K : A -n> (IT -n> IT)) (k : A -n> IT) : *)
-  (*   A -n> (IT -n> IT) := *)
-  (*   λne env t, interp_throw (λne env, K env t) k env. *)
-  (* Solve All Obligations with solve_proper_please. *)
-
-  (* Program Definition interp_throwrk {A} (e : A -n> IT) (K : A -n> (IT -n> IT)) : *)
-  (*   A -n> (IT -n> IT) := *)
-  (*   λne env t, interp_throw e (λne env, K env t) env. *)
-  (* Solve All Obligations with solve_proper_please. *)
+  #[local] Instance interp_reset_full_ne {S} (f : @interp_scope F R _ S -n> IT):
+    NonExpansive (λ env, interp_reset (f env)).
+  Proof. solve_proper. Qed.
 
   (** Interpretation for all the syntactic categories: values, expressions, contexts *)
   Fixpoint interp_val {S} (v : val S) : interp_scope S -n> IT :=
@@ -555,17 +653,10 @@ Section interp.
     | App e1 e2 => interp_app (interp_expr e1) (interp_expr e2)
     | NatOp op e1 e2 => interp_natop op (interp_expr e1) (interp_expr e2)
     | If e e1 e2 => interp_if (interp_expr e) (interp_expr e1) (interp_expr e2)
-    | Input => interp_input
-    | Output e => interp_output (interp_expr e)
     | Shift e => interp_shift (interp_expr e)
-    | Reset e => interp_reset (interp_expr e)
+    | Reset e => λne env, (OfeMor interp_reset) (interp_expr e env)
     end.
-  Solve All Obligations with first [ solve_proper | solve_proper_please ].
 
-
-  Program Definition interp_outputk {A} : (A -n> IT) -n> A -n> IT :=
-    λne t env, interp_output t env.
-  Solve All Obligations with solve_proper.
 
   Program Definition interp_apprk {A} (q : A -n> IT) : (A -n> IT) -n> A -n> IT :=
     λne t env, interp_app q t env.
@@ -590,31 +681,19 @@ Section interp.
   λne b env, interp_if b e1 e2 env.
   Solve All Obligations with solve_proper.
 
-  (* Program Definition interp_iftruek {A} (b e2 : A -n> IT) : *)
-  (*   (A -n> IT) -n> A -n> IT := *)
-  (* λne e1 env, interp_if b e1 e2 env. *)
-  (* Solve All Obligations with solve_proper. *)
-
-  (* Program Definition interp_iffalsek {A} (b e1 : A -n> IT) : *)
-  (*   (A -n> IT) -n> A -n> IT := *)
-  (* λne e2 env, interp_if b e1 e2 env. *)
-  (* Solve All Obligations with solve_proper. *)
 
   Program Definition interp_resetk {A} : (A -n> IT) -n> A -n> IT :=
-    λne t env, interp_reset t env.
+    λne t env, interp_reset (t env).
   Solve All Obligations with solve_proper.
 
   Definition interp_ectx_el {S} (C : ectx_el S) :
     (interp_scope S -n> IT) -n> (interp_scope S) -n> IT :=
     match C with
-    | OutputK => interp_outputk
     | AppRK e1 => interp_apprk (interp_expr e1)
     | AppLK e2 => interp_applk (interp_expr e2)
     | NatOpRK op e1 => interp_natoprk op (interp_expr e1)
     | NatOpLK op e2 => interp_natoplk op (interp_expr e2)
     | IfK e1 e2 => interp_ifk (interp_expr e1) (interp_expr e2)
-    (* | IfTrueK b e2 => interp_iftruek (interp_expr b) (interp_expr e2) *)
-    (* | IfFalseK b e1 => interp_iffalsek (interp_expr b) (interp_expr e1) *)
     | ResetK => interp_resetk
     end.
 
@@ -652,7 +731,6 @@ Section interp.
   Definition interp_ectx {S} (K : ectx S) : interp_scope S -n> (IT -n> IT) :=
     OfeMor (interp_ectx'' K).
 
-  Example test_ectx : ectx ∅ := [OutputK ; AppRK (RecV (Var VZ))].
   (* Eval cbv[test_ectx interp_ectx interp_ectx' interp_ectx_el *)
   (*            interp_apprk interp_outputk interp_output interp_app] in (interp_ectx test_ectx). *)
   (* Definition interp_ectx {S} (K : ectx S) : interp_scope S -n> IT -n> IT := *)
@@ -704,14 +782,9 @@ Section interp.
   (*   interp_ectx (fmap δ e) env ≡ interp_ectx e (ren_scope δ env). *)
   Proof.
     - destruct e; simpl; try by repeat f_equiv.
-      (* repeat f_equiv. *)
-      (* intros ?; simpl. *)
-      (* repeat f_equiv. *)
-      (* simpl; rewrite interp_expr_ren. *)
-      (* f_equiv. *)
-      (* intros [| y]; simpl. *)
-      (* + reflexivity. *)
-      (* + reflexivity. *)
+      + repeat f_equiv. by repeat (intro; simpl; repeat f_equiv).
+      + unfold interp_reset. repeat f_equiv.
+        by repeat (intro; simpl; repeat f_equiv).
     - destruct e; simpl.
       + reflexivity.
       + clear -interp_expr_ren.
@@ -779,16 +852,8 @@ Section interp.
   (*   interp_ectx (bind δ e) env ≡ interp_ectx e (sub_scope δ env). *)
   Proof.
     - destruct e; simpl; try by repeat f_equiv.
-      (* repeat f_equiv. *)
-      (* intros ?; simpl. *)
-      (* repeat f_equiv. *)
-      (* rewrite interp_expr_subst. *)
-      (* f_equiv. *)
-      (* intros [| x']; simpl. *)
-      (* + reflexivity. *)
-      (* + rewrite interp_expr_ren. *)
-      (*   f_equiv. *)
-      (*   intros ?; reflexivity. *)
+      + repeat f_equiv. by repeat (intro; simpl; repeat f_equiv).
+      + unfold interp_reset; repeat f_equiv. by repeat (intro; simpl; repeat f_equiv).
     - destruct e; simpl.
       + reflexivity.
       + clear -interp_expr_subst.
@@ -838,17 +903,6 @@ Section interp.
     by rewrite laterO_map_id.
   Qed.
 
-  #[global] Instance interp_ectx_hom_output {S} (K : ectx S) env :
-    IT_hom (interp_ectx K env) ->
-    IT_hom (interp_ectx (OutputK :: K) env).
-  Proof.
-    intros. simple refine (IT_HOM _ _ _ _ _); intros; simpl.
-    - by rewrite !hom_tick.
-    - rewrite !hom_vis.
-      f_equiv. intro. simpl. rewrite -laterO_map_compose.
-      do 2 f_equiv. by intro.
-    - by rewrite !hom_err.
-  Qed.
 
   #[global] Instance interp_ectx_hom_if {S}
     (K : ectx S) (e1 e2 : expr S) env :
@@ -926,18 +980,32 @@ Section interp.
   Qed.
 
   (* ResetK is not a homomorphism *)
-  Lemma interp_ectx_reset_not_hom {S} env :
-    IT_hom (interp_ectx ([ResetK] : ectx S) env) -> False.
+  (* Lemma interp_ectx_reset_not_hom {S} env : *)
+  (*   IT_hom (interp_ectx ([ResetK] : ectx S) env) -> False. *)
+  (* Proof. *)
+  (*   intros [ _ Hi _ _ ]. simpl in Hi. *)
+  (*   specialize (Hi (Ret 0)). *)
+  (*   unfold interp_reset, CALLCC, CALLCC_ in Hi. *)
+  (*   simpl in Hi. *)
+  (*   apply bi.siProp.pure_soundness. *)
+  (*   iApply IT_tick_vis_ne. *)
+  (*   iPureIntro. *)
+  (*   symmetry. *)
+  (*   eapply Hi. *)
+  (*   Unshelve. apply bi.siProp_internal_eq. *)
+  (* Qed. *)
+
+  #[global] Instance interp_ectx_hom_reset {S} (K : ectx S)
+    (env : interp_scope S) :
+    IT_hom (interp_ectx K env) ->
+    IT_hom (interp_ectx (ResetK :: K) env).
   Proof.
-    intros [ _ Hi _ _ ]. simpl in Hi.
-    specialize (Hi (Ret 0)).
-    rewrite hom_vis in Hi.
-    apply bi.siProp.pure_soundness.
-    iApply IT_tick_vis_ne.
-    iPureIntro.
-    symmetry.
-    eapply Hi.
-    Unshelve. apply bi.siProp_internal_eq.
+    intros H. simple refine (IT_HOM _ _ _ _ _); intros; simpl; unfold interp_reset.
+
+    - rewrite -hom_tick. f_equiv. by rewrite get_val_tick.
+    - rewrite get_val_vis. rewrite hom_vis. f_equiv.
+      intro. simpl. rewrite -laterO_map_compose. done.
+    - by rewrite get_val_err hom_err.
   Qed.
 
 
@@ -950,21 +1018,18 @@ Section interp.
 
   #[global] Instance interp_ectx_hom {S}
     (K : ectx S) env :
-    ResetK ∉ K ->
     IT_hom (interp_ectx K env).
   Proof.
-    intro.
     induction K; simpl; first apply IT_hom_idfun.
-    apply not_elem_of_cons in H. destruct H as [H1 ?]. specialize (IHK H).
-    destruct a; try apply _. contradiction.
+    destruct a; apply _.
   Qed.
 
   (** ** Finally, preservation of reductions *)
-  Lemma interp_expr_head_step {S : Set} (env : interp_scope S) (e : expr S) e' σ σ' K Ko n :
-    head_step e σ K e' σ' K Ko (n, 0) →
+  Lemma interp_expr_head_step {S : Set} (env : interp_scope S) (e : expr S) e' K K' Ko n :
+    head_step e K e' K' Ko (n, 0) →
     interp_expr e env ≡ Tick_n n $ interp_expr e' env.
   Proof.
-    inversion 1; cbn-[IF APP' INPUT Tick get_ret2].
+    inversion 1; cbn-[IF APP' Tick get_ret2].
     - (* app lemma *)
       subst.
       erewrite APP_APP'_ITV; last apply _.
@@ -996,34 +1061,72 @@ Section interp.
       reflexivity.
   Qed.
 
-  Lemma interp_expr_fill_no_reify {S} K K' Ko (env : interp_scope S) (e e' : expr S) σ σ' n :
-    head_step e σ K e' σ' K' Ko (n, 0) →
-    ResetK ∉ K->
-    interp_expr (fill K e) env ≡ Tick_n n $ interp_expr (fill K' e') env.
+  Lemma interp_expr_fill_no_reify {S} (env : interp_scope S) (e e' : expr S) n :
+    prim_step e e' (n, 0) →
+    interp_expr e env ≡ Tick_n n $ interp_expr e' env.
   Proof.
-    inversion 1; subst; intros H1; rewrite !interp_comp;
-      apply (interp_ectx_hom K' env) in H1.
-    - rewrite <-hom_tick_n; last eauto.
-      simpl. apply (interp_expr_head_step env) in H.
-      by rewrite equiv_dist => n; f_equiv; move : n; apply equiv_dist.
-    - rewrite <-hom_tick_n; last eauto. apply (interp_expr_head_step env) in H.
-      by rewrite H.
-    - rewrite <-hom_tick_n; last eauto. apply (interp_expr_head_step env) in H.
-      by rewrite H.
-    - rewrite <-hom_tick_n; last eauto. apply (interp_expr_head_step env) in H.
-      by rewrite H.
-    - rewrite <-hom_tick_n; last eauto. apply (interp_expr_head_step env) in H.
-      by rewrite H.
+    inversion 1; subst.
+    inversion H1; subst; rewrite !interp_comp; simpl.
+    - rewrite -hom_tick. rewrite -(shift_context_app K Ki' Ko); eauto.
+      f_equiv. eapply (interp_expr_head_step env _ _ _ _ _) in H1.
+      simpl in H1. done.
+    - rewrite -!hom_tick. rewrite -(shift_context_app K Ki' Ko); eauto.
+      f_equiv. eapply (interp_expr_head_step env _ _ _ _ _) in H1.
+      simpl in H1. done.
+    - rewrite -(shift_context_app K Ki' Ko); eauto.
+      f_equiv. eapply (interp_expr_head_step env _ _ _ _ _) in H1.
+      simpl in H1. done.
+    - rewrite -(shift_context_app K Ki' Ko); eauto.
+      f_equiv. eapply (interp_expr_head_step env _ _ _ _ _) in H1.
+      simpl in H1. done.
+    - rewrite -(shift_context_app K Ki' Ko); eauto.
+      f_equiv. eapply (interp_expr_head_step env _ _ _ _ _) in H1.
+      simpl in H1. done.
   Qed.
 
-  Opaque INPUT OUTPUT_ SHIFT RESET.
   Opaque extend_scope.
   Opaque Ret.
 
+
+
+  Parameter env : @interp_scope F R CR ∅.
+  Parameter σ : state.
+  Parameter (σr : gState_rest sR_idx rs ♯ IT).
+  Example term : expr ∅ := ((#2) + reset ((#3) + shift/cc (rec (($0) ⋆ (# 5)))))%syn.
+  (* Goal forall e, (interp_expr term env) ≡ e -> *)
+  (*   exists e' σ', reify (gReifiers_sReifier rs) *)
+  (*               e (gState_recomp σr (sR_state σ)) ≡ (gState_recomp σr (sR_state σ'), e'). *)
+  (* Proof. *)
+  (*   intros. *)
+  (*   eexists. eexists. Opaque CALLCC_. simpl in H. *)
+  (*   rewrite /interp_reset in H. *)
+  (*   rewrite !hom_CALLCC_ in H. *)
+  (*   match goal with *)
+  (*   | H : (equiv ?f e) |- _ => set (g := f) *)
+  (*   end. *)
+  (*   trans (reify (gReifiers_sReifier rs) g (gState_recomp σr (sR_state σ))). *)
+  (*   { f_equiv. f_equiv. symmetry. apply H. } *)
+  (*   subst g. *)
+  (*   rewrite reify_vis_eq //; first last. *)
+  (*   match goal with *)
+  (*   | |- context G [ofe_mor_car _ _ (sReifier_re _ _) (?f, _, ?h)] => set (i := f); set (o := h) *)
+  (*   end. *)
+  (*   epose proof (@subReifier_reify sz reify_delim rs _ IT _ op_callcc (subEff_ins^-1 i) _ (o ◎ subEff_outs) σ _ σr) as He. *)
+  (*   simpl in He |-*. *)
+  (*   erewrite <-He; last reflexivity. *)
+  (*   f_equiv. *)
+  (*   - intros [][][]. simpl. solve_proper. *)
+  (*   - f_equiv. f_equiv. *)
+  (*     + f_equiv. by rewrite ofe_iso_21. *)
+  (*     + intro. simpl. rewrite ofe_iso_12. done. *)
+
+
   Lemma interp_expr_fill_yes_reify {S} K K' Ko env (e e' : expr S)
-    (σ σ' : stateO) (σr : gState_rest sR_idx rs ♯ IT) n :
-    head_step e σ K e' σ' K' Ko (n, 1) →
-    ResetK ∉ K->
+    (σ σ' : state)
+    (σr : gState_rest sR_idx rs ♯ IT) n :
+    head_step e K e' K' Ko (n, 1) →
+    some_relation K Ko σ ->
+    some_relation K' Ko σ ->
     reify (gReifiers_sReifier rs)
       (interp_expr (fill K e) env) (gState_recomp σr (sR_state σ))
       ≡ (gState_recomp σr (sR_state σ'), Tick_n n $ interp_expr (fill K' e') env).
