theories/input_lang_delim/lang.v
@@ -21,8 +21,8 @@ Inductive expr {X : Set} :=
 | NatOp (op : nat_op) (e₁ : expr) (e₂ : expr) : expr
 | If (e₁ : expr) (e₂ : expr) (e₃ : expr) : expr
 (* The effects *)
-| Input : expr
-| Output (e : expr) : expr
+(* | Input : expr *)
+(* | Output (e : expr) : expr *)
 | Shift (e : expr) : expr
 | Reset (e : expr) : expr
 with val {X : Set} :=
@@ -33,7 +33,7 @@ with val {X : Set} :=
 
 
 Variant ectx_el {X : Set} :=
-  | OutputK : ectx_el
+  (* | OutputK : ectx_el *)
   | IfK (e1 : @expr X) (e2 : @expr X) : ectx_el
   | AppLK (v : @val X) : ectx_el (* ◻ v *)
   | AppRK (e : @expr X) : ectx_el (* e ◻ *)
@@ -62,8 +62,8 @@ Fixpoint emap {A B : Set} (f : A [→] B) (e : expr A) : expr B :=
   | App e₁ e₂ => App (emap f e₁) (emap f e₂)
   | NatOp o e₁ e₂ => NatOp o (emap f e₁) (emap f e₂)
   | If e₁ e₂ e₃ => If (emap f e₁) (emap f e₂) (emap f e₃)
-  | Input => Input
-  | Output e => Output (emap f e)
+  (* | Input => Input *)
+  (* | Output e => Output (emap f e) *)
   | Shift e => Shift (emap f e)
   | Reset e => Reset (emap f e)
   end
@@ -80,7 +80,7 @@ vmap {A B : Set} (f : A [→] B) (v : val A) : val B :=
 
 Definition kmap {A B : Set} (f : A [→] B) (K : ectx A) : ectx B :=
   map (fun x => match x with
-              | OutputK => OutputK
+              (* | OutputK => OutputK *)
               | IfK e1 e2 => IfK (fmap f e1) (fmap f e2)
               | AppLK v => AppLK (fmap f v)
               | AppRK e => AppRK (fmap f e)
@@ -100,8 +100,8 @@ Fixpoint ebind {A B : Set} (f : A [⇒] B) (e : expr A) : expr B :=
   | App e₁ e₂ => App (ebind f e₁) (ebind f e₂)
   | NatOp o e₁ e₂ => NatOp o (ebind f e₁) (ebind f e₂)
   | If e₁ e₂ e₃ => If (ebind f e₁) (ebind f e₂) (ebind f e₃)
-  | Input => Input
-  | Output e => Output (ebind f e)
+  (* | Input => Input *)
+  (* | Output e => Output (ebind f e) *)
   | Shift e => Shift (ebind f e)
   | Reset e => Reset (ebind f e)
   end
@@ -118,7 +118,7 @@ vbind {A B : Set} (f : A [⇒] B) (v : val A) : val B :=
 
 Definition kbind {A B : Set} (f : A [⇒] B) (K : ectx A) : ectx B :=
   map (fun x => match x with
-              | OutputK => OutputK
+              (* | OutputK => OutputK *)
               | IfK e1 e2 => IfK (bind f e1) (bind f e2)
               | AppLK v => AppLK (bind f v)
               | AppRK e => AppRK (bind f e)
@@ -355,7 +355,7 @@ Definition nat_op_interp {S} (n : nat_op) (x y : val S) : option (val S) :=
 
 Definition ctx_el_to_expr {X : Set} (K : ectx_el X) (e : expr X) : expr X :=
   match K with
-  | OutputK => Output $ e
+  (* | OutputK => Output $ e *)
   | IfK e1 e2 => If e e1 e2
   | AppLK v => App e (Val v)
   | AppRK el => App el e
@@ -388,6 +388,8 @@ Definition shift_context {X : Set} (K : ectx X) : (ectx X * ectx X) :=
   let (Ki, Ko) := trim_to_first_reset K [] in
   (List.rev Ki, Ko).
 
+
+
 Lemma trim_to_first_reset_app {X : Set} (K Ki Ko acc : ectx X) :
   (Ki, Ko) = trim_to_first_reset K acc ->
   (List.rev Ki) ++ Ko = (List.rev acc) ++ K.
@@ -399,7 +401,6 @@ Proof.
                   rewrite -app_assoc; symmetry; apply cons_middle).
     by inversion H.
 Qed.
-
 
 
 Lemma shift_context_app {X : Set} (K Ki Ko : ectx X) :
@@ -458,7 +459,7 @@ Qed.
 Definition cont_to_rec {X : Set} (K : ectx X) : (val X) :=
   ContV (fill (shift K) (Var VZ)).
 
-Example test1 : val (inc ∅) := (cont_to_rec [OutputK; AppRK (Var VZ)]).
+Example test1 : val (inc ∅) := (cont_to_rec [(NatOpLK Add (LitV 3)); AppRK (Var VZ)]).
 
 (* Lemma fill_emap {X Y : Set} (f : X [→] Y) (K : ectx X) (e : expr X) *)
 (*   : fmap f (fill K e) = fill (fmap f K) (fmap f e). *)
@@ -472,68 +473,66 @@ Example test1 : val (inc ∅) := (cont_to_rec [OutputK; AppRK (Var VZ)]).
 
 (*** Operational semantics *)
 
-Record state := State {
-                   inputs : list nat;
-                   outputs : list nat;
-                 }.
-#[export] Instance state_inhabited : Inhabited state := populate (State [] []).
+(* Record state := State { *)
+(*                     inputs : list nat; *)
+(*                     outputs : list nat; *)
+(*                  }. *)
+(* #[export] Instance state_inhabited : Inhabited state := populate (State [] []). *)
 
-Definition update_input (s : state) : nat * state :=
-  match s.(inputs) with
-  | [] => (0, s)
-  | n::ns =>
-      (n, {| inputs := ns; outputs := s.(outputs) |})
-  end.
-Definition update_output (n:nat) (s : state) : state :=
-  {| inputs := s.(inputs); outputs := n::s.(outputs) |}.
+(* Definition update_input (s : state) : nat * state := *)
+(*   match s.(inputs) with *)
+(*   | [] => (0, s) *)
+(*   | n::ns => *)
+(*       (n, {| inputs := ns; outputs := s.(outputs) |}) *)
+(*   end. *)
+(* Definition update_output (n:nat) (s : state) : state := *)
+(*   {| inputs := s.(inputs); outputs := n::s.(outputs) |}. *)
 
 
 (** [head_step e σ K e' σ' K' Ko (n, m)] : step from [(e, σ, K)] to [(e', σ', K')]
     under outer context [Ko] in [n] ticks with [m] effects encountered *)
-Variant head_step {S} : expr S -> state -> ectx S ->
-                        expr S -> state -> ectx S ->
+Variant head_step {S} : expr S -> ectx S ->
+                        expr S -> ectx S ->
                         ectx S ->
                         nat * nat → Prop :=
-  | BetaS e1 v2 σ K Ko :
-    head_step (App (Val $ RecV e1) (Val v2)) σ K
+  | BetaS e1 v2 K Ko :
+    head_step (App (Val $ RecV e1) (Val v2)) K
       (subst (Inc := inc) ((subst (F := expr) (Inc := inc) e1)
                              (Val (shift (Inc := inc) v2)))
-         (Val (RecV e1))) σ K Ko (1,0)
-  | BetaContS e1 v2 σ K Ko :
-    head_step (App (Val $ ContV e1) (Val v2)) σ K
+         (Val (RecV e1))) K Ko (1,0)
+  | BetaContS e1 v2 K Ko :
+    head_step (App (Val $ ContV e1) (Val v2)) K
       (subst  (Inc := inc) e1 (Val  v2))
-      σ K Ko (2,0)
-  | InputS σ n σ' K Ko :
-    update_input σ = (n, σ') →
-    head_step Input σ K (Val (LitV n)) σ' K Ko (1, 1)
-  | OutputS σ n σ' K Ko :
-    update_output n σ = σ' →
-    head_step (Output (Val (LitV n))) σ K (Val (LitV 0)) σ' K Ko (1, 1)
-  | NatOpS op v1 v2 v3 σ K Ko :
+      K Ko (2,0)
+  (* | InputS n σ' K Ko : *)
+  (*   update_input = (n, σ') → *)
+  (*   head_step Input K (Val (LitV n)) σ' K Ko (1, 1) *)
+  (* | OutputS n σ' K Ko : *)
+  (*   update_output n = σ' → *)
+  (*   head_step (Output (Val (LitV n))) K (Val (LitV 0)) σ' K Ko (1, 1) *)
+  | NatOpS op v1 v2 v3 K Ko :
     nat_op_interp op v1 v2 = Some v3 →
-    head_step (NatOp op (Val v1) (Val v2)) σ K
-      (Val v3) σ K Ko (0, 0)
-  | IfTrueS n e1 e2 σ K Ko :
+    head_step (NatOp op (Val v1) (Val v2)) K
+      (Val v3) K Ko (0, 0)
+  | IfTrueS n e1 e2 K Ko :
     n > 0 →
-    head_step (If (Val (LitV n)) e1 e2) σ K
-      e1 σ K Ko (0, 0)
-  | IfFalseS n e1 e2 σ K Ko :
+    head_step (If (Val (LitV n)) e1 e2) K
+      e1 K Ko (0, 0)
+  | IfFalseS n e1 e2 K Ko :
     n = 0 →
-    head_step (If (Val (LitV n)) e1 e2) σ K
-      e2 σ K Ko (0, 0)
+    head_step (If (Val (LitV n)) e1 e2) K
+      e2 K Ko (0, 0)
 
-  | ShiftS (e : expr (inc (inc S))) σ K Ko f :
+  | ShiftS (e : expr (inc (inc S))) K Ko f :
     ResetK ∉ K ->
-    f = cont_to_rec K ->
-    head_step (Shift (Val $ RecV e)) σ K
+    f = cont_to_rec (ResetK::K) ->
+    head_step (Shift (Val $ RecV e)) K
       (subst (Inc := inc) ((subst (F := expr) (Inc := inc) e)
                              (Val (shift (Inc := inc) f)))
-         (Val $ RecV e)) σ [] Ko (1, 1)
-    (* head_step (Shift  (Val $ RecV e)) σ K *)
-    (*           (App (Val $ RecV e) (Val f)) σ [] (0, 1) *)
+         (Val $ RecV e)) [] Ko (1, 1)
 
-  | ResetS v σ K Ko :
-    head_step (Reset (Val v)) σ K (Val v) σ K Ko (1, 1).
+  | ResetS v K Ko :
+    head_step (Reset (Val v)) K (Val v) K Ko (1, 1).
 
 
   (* | ValueS v σ K C: *)
@@ -544,15 +543,15 @@ Variant head_step {S} : expr S -> state -> ectx S ->
   (*     (Reset (fill E (Shift e))) σ *)
   (*     (Reset (subst (Inc := inc) e (Val $ ContV $ ResetK E))) σ K (1,0). *)
 
-Lemma head_step_io_01 {S} (e1 e2 : expr S) σ1 σ2 K K' Ko n m :
-  head_step e1 σ1 K e2 σ2 K' Ko (n,m) → m = 0 ∨ m = 1.
+Lemma head_step_io_01 {S} (e1 e2 : expr S) K K' Ko n m :
+  head_step e1 K e2 K' Ko (n,m) → m = 0 ∨ m = 1.
 Proof.  inversion 1; eauto. Qed.
 (* Lemma head_step_unfold_01 {S} (e1 e2 : expr S) σ1 σ2 K K' n m : *)
 (*   head_step e1 σ1 K e2 σ2 K' (n,m) → n = 0 ∨ n = 1. *)
 (* Proof.  inversion 1; eauto. Qed. *)
-Lemma head_step_no_io {S} (e1 e2 : expr S) σ1 σ2 K K' Ko n :
-  head_step e1 σ1 K e2 σ2 K' Ko (n,0) → σ1 = σ2.
-Proof.  inversion 1; eauto. Qed.
+(* Lemma head_step_no_io {S} (e1 e2 : expr S) σ1 σ2 K K' Ko n : *)
+(*   head_step e1 σ1 K e2 σ2 K' Ko (n,0) → σ1 = σ2. *)
+(* Proof.  inversion 1; eauto. Qed. *)
 
 (** Carbonara from heap lang *)
 
@@ -573,8 +572,8 @@ Proof. elim: Ki e; simpl in *; first done. intros.
 Qed.
 
 (* CHECK *)
-Lemma val_head_stuck {S} (e1 : expr S) σ1 e2 σ2 K K' Ko m :
-  head_step e1 σ1 K e2 σ2 K' Ko m → to_val e1 = None.
+Lemma val_head_stuck {S} (e1 : expr S) e2 K K' Ko m :
+  head_step e1 K e2 K' Ko m → to_val e1 = None.
 Proof. destruct 1; naive_solver. Qed.
 
 
@@ -601,47 +600,47 @@ Proof. by rewrite fill_app. Qed.
 
 
 (* FIXME maybe *)
-Inductive prim_step {S} : ∀ (e1 : expr S) (σ1 : state)
-          (e2 : expr S) (σ2 : state) (nm : nat * nat), Prop :=
+Inductive prim_step {S} : ∀ (e1 : expr S) 
+          (e2 : expr S) (nm : nat * nat), Prop :=
 (* | Ectx_step e1 σ1 e2 σ2 nm (K1 K2 : ectx S) e1' e2' : *)
 (*   e1 = fill K1 e1' -> *)
 (*   e2 = fill K2 e2' -> *)
 (*   ResetK ∉ K1 -> *)
 (*   head_step e1' σ1 K1 e2' σ2 K2 nm -> *)
 (*   prim_step e1 σ1 e2 σ2 nm *)
-| Shift_step e1 σ1 K Ki Ko e2 σ2 Ki' nm :
+| Shift_step e1 K Ki Ko e2 Ki' nm :
   (Ki, Ko) = shift_context K ->
-  head_step e1 σ1 Ki e2 σ2 Ki' Ko nm ->
-  prim_step (fill K e1) σ1 (fill (Ki' ++ Ko) e2) σ2 nm.
+  head_step e1 Ki e2 Ki' Ko nm ->
+  prim_step (fill K e1) (fill (Ki' ++ Ko) e2) nm.
 (* CHECK *)
 
-Lemma prim_step_pure {S} (e1 e2 : expr S) σ1 σ2 n :
-  prim_step e1 σ1 e2 σ2 (n,0) → σ1 = σ2.
-Proof.
-  inversion 1; simplify_eq/=. by inversion H1.
-Qed.
+(* Lemma prim_step_pure {S} (e1 e2 : expr S) σ1 σ2 n : *)
+(*   prim_step e1 σ1 e2 σ2 (n,0) → σ1 = σ2. *)
+(* Proof. *)
+(*   inversion 1; simplify_eq/=. by inversion H1. *)
+(* Qed. *)
 
-Inductive prim_steps {S} : expr S → state → expr S → state → nat * nat → Prop :=
-| prim_steps_zero e σ :
-  prim_steps e σ e σ (0, 0)
-| prim_steps_abit e1 σ1 e2 σ2 e3 σ3 n1 m1 n2 m2 :
-  prim_step e1 σ1 e2 σ2 (n1, m1) →
-  prim_steps e2 σ2 e3 σ3 (n2, m2) →
-  prim_steps e1 σ1 e3 σ3 (plus n1 n2, plus m1 m2)
+Inductive prim_steps {S} : expr S → expr S → nat * nat → Prop :=
+| prim_steps_zero e :
+  prim_steps e e (0, 0)
+| prim_steps_abit e1 e2 e3 n1 m1 n2 m2 :
+  prim_step e1 e2 (n1, m1) →
+  prim_steps e2 e3 (n2, m2) →
+  prim_steps e1 e3 (plus n1 n2, plus m1 m2)
 .
 
-Lemma Ectx_step' {S} (K1 K2 : ectx S) e1 σ1 e2 σ2 efs :
-  head_step e1 σ1 K1 e2 σ2 K2 [] efs →
+Lemma Ectx_step' {S} (K1 K2 : ectx S) e1 e2 efs :
+  head_step e1 K1 e2 K2 [] efs →
   ResetK ∉ K1 ->
-  prim_step (fill K1 e1) σ1 (fill K2 e2) σ2 efs.
+  prim_step (fill K1 e1) (fill K2 e2) efs.
 Proof.
   intros. rewrite -(app_nil_r K2).
   econstructor; eauto. by apply no_reset_shift_context_ident.
 Qed.
 
-Lemma prim_steps_app {S} nm1 nm2 (e1 e2 e3 : expr S) σ1 σ2 σ3 :
-  prim_steps e1 σ1 e2 σ2 nm1 → prim_steps e2 σ2 e3 σ3 nm2 →
-  prim_steps e1 σ1 e3 σ3 (plus nm1.1 nm2.1, plus nm1.2 nm2.2).
+Lemma prim_steps_app {S} nm1 nm2 (e1 e2 e3 : expr S) :
+  prim_steps e1 e2 nm1 → prim_steps e2 e3 nm2 →
+  prim_steps e1 e3 (plus nm1.1 nm2.1, plus nm1.2 nm2.2).
 Proof.
   intros Hst. revert nm2.
   induction Hst; intros [n' m']; simplify_eq/=; first done.
@@ -650,8 +649,8 @@ Proof.
   by apply (IHHst (n',m')).
 Qed.
 
-Lemma prim_step_steps {S} nm (e1 e2 : expr S) σ1 σ2 :
-  prim_step e1 σ1 e2 σ2 nm → prim_steps e1 σ1 e2 σ2 nm.
+Lemma prim_step_steps {S} nm (e1 e2 : expr S) :
+  prim_step e1 e2 nm → prim_steps e1 e2 nm.
 Proof.
   destruct nm as [n m]. intro Hs.
   rewrite -(Nat.add_0_r n).
@@ -660,20 +659,132 @@ Proof.
   by constructor.
 Qed.
 
-Lemma prim_step_steps_steps {S} (e1 e2 e3 : expr S) σ1 σ2 σ3 nm1 nm2 nm3 :
+Lemma prim_step_steps_steps {S} (e1 e2 e3 : expr S) nm1 nm2 nm3 :
   nm3 = (plus nm1.1 nm2.1, plus nm1.2 nm2.2) ->
-  prim_step e1 σ1 e2 σ2 nm1 → prim_steps e2 σ2 e3 σ3 nm2 -> prim_steps e1 σ1 e3 σ3 nm3.
+  prim_step e1 e2 nm1 → prim_steps e2 e3 nm2 -> prim_steps e1 e3 nm3.
 Proof.
   intros -> H G.
   eapply prim_steps_app; last apply G.
   apply prim_step_steps, H.
 Qed.
 
-Lemma head_step_prim_step {S} (e1 e2 : expr S) σ1 σ2 nm :
-  head_step e1 σ1 [] e2 σ2 [] [] nm -> prim_step e1 σ1 e2 σ2 nm.
+Lemma head_step_prim_step {S} (e1 e2 : expr S) nm :
+  head_step e1 [] e2 [] [] nm -> prim_step e1 e2 nm.
 Proof.
   move => H; apply Ectx_step' in H => //=. apply not_elem_of_nil.
 Qed.
+
+
+(*** Abstract Machine semantics *)
+
+Definition Mectx {S} := list $ ectx S.
+
+Variant config {S} : Type :=
+  | Ceval : expr S -> ectx S -> @Mectx S -> config
+  | Ccont : ectx S -> val S -> @Mectx S -> config
+  | Cmcont : @Mectx S -> val S -> config
+  | Cexpr : expr S -> config
+  | Cret : val S -> config.
+
+Reserved Notation "c '===>' c' / nm"
+  (at level 40, c', nm at level 30).
+
+Variant Cred {S : Set} : config -> config -> (nat * nat) -> Prop :=
+
+  (* init *)
+  | Ceval_init : forall (e : expr S),
+      Cexpr e ===> Ceval e [] [] / (0,0)
+
+  (* eval *)
+  | Ceval_val : forall v k mk,
+      Ceval (Val v) k mk ===> Ccont k v mk / (0,0)
+
+  | Ceval_app : forall e0 e1 k mk,
+      Ceval (App e0 e1) k mk ===> Ceval e1 (AppRK e0 :: k) mk / (0,0)
+
+  | Ceval_natop : forall op e0 e1 k mk,
+      Ceval (NatOp op e0 e1) k mk ===> Ceval e1 (NatOpRK op e0 :: k) mk / (0,0)
+
+  | Ceval_if : forall eb et ef k mk,
+      Ceval (If eb et ef) k mk ===> Ceval eb (IfK et ef :: k) mk / (0,0)
+
+  | Ceval_reset : forall e k mk,
+      Ceval (Reset e) k mk ===> Ceval e [] (k :: mk) / (1, 1)
+
+  | Ceval_shift : forall (e : expr $ inc $ inc S) k f mk,
+      f = cont_to_rec (k) ->    (* CHECK: should we add a reset to ctx ? don't think so *)
+      Ceval (Shift $ Val $ RecV e) k mk ===>
+        Ceval (subst (Inc := inc)
+                 (subst (F := expr) (Inc := inc)
+                    e (Val (shift (Inc:=inc) f)))
+                 (Val (RecV e))) [] mk / (1, 1)
+
+  (* cont *)
+  | Ccont_hole : forall v mk,
+      Ccont [] v mk ===> Cmcont mk v / (0,0)
+
+  | Ccont_appr : forall e v k mk,
+      Ccont (AppRK e :: k) v mk ===> Ceval e (AppLK v :: k) mk / (0, 0)
+
+  | Ccont_appl : forall e v k mk,
+      Ccont (AppLK v :: k) (RecV e) mk ===>
+        Ceval (subst (Inc := inc)
+                 (subst (F := expr) (Inc := inc) e
+                    (Val (shift (Inc := inc) v)))
+                 (Val (RecV e))) k mk / (1, 0)
+
+  | Ccont_cont : forall e v k mk,
+      Ccont (AppLK v :: k) (ContV e) mk ===>
+        Ceval (subst (Inc := inc) e (Val v)) [] (k :: mk) / (2, 0)
+
+  | Ccont_ift : forall et ef n k mk,
+      n > 0 ->
+      Ccont (IfK et ef :: k) (LitV n) mk ===>
+        Ceval et k mk / (0, 0)
+
+  | Ccont_iff : forall et ef n k mk,
+      n = 0 ->
+      Ccont (IfK et ef :: k) (LitV n) mk ===>
+        Ceval ef k mk / (0, 0)
+
+  | Ccont_natopr : forall op e v k mk,
+      Ccont (NatOpRK op e :: k) v mk ===>
+        Ceval e (NatOpLK op v :: k) mk / (0, 0)
+
+  | Ccont_natopl : forall op v0 v1 v2 k mk,
+      nat_op_interp op v0 v1 = Some v2 ->
+      Ccont (NatOpLK op v1 :: k) v0 mk ===>
+        Ceval (Val v2) k mk / (0,0)
+
+
+  (* meta-cont *)
+  | Cmcont_cont : forall k mk v,
+      Cmcont (k :: mk) v ===> Ccont k v mk / (0,0)
+
+  | Cmcont_ret : forall v,
+      Cmcont [] v ===> Cret v / (0, 0)
+
+where "c ===> c' / nm" := (Cred c c' nm).
+
+Arguments Mectx S%bind : clear implicits.
+Arguments config S%bind : clear implicits.
+
+(** ** On configs & meta-contexts *)
+
+Definition meta_fill {S} (mk : Mectx S) e :=
+  fold_left (λ e k, fill k e) mk e.
+
+
+Definition config_to_expr {S} (c : config S) :=
+  match c with
+  | Ceval e k mk => meta_fill mk (fill k e)
+  | Ccont k v mk => meta_fill mk (fill k (Val v))
+  | Cmcont mk v => meta_fill mk (Val v)
+  | Cexpr e => e
+  | Cret v => Val v
+  end.
+(* i mean not really bcause missing [reset]s *)
+
 
 (*** Type system *)
 
@@ -700,11 +811,11 @@ Inductive typed {S : Set} (Γ : S -> ty) : expr S → ty → Prop :=
   typed Γ e1 τ →
   typed Γ e2 τ →
   typed Γ (If e0 e1 e2) τ
-| typed_Input :
-  typed Γ Input Tnat
-| typed_Output e :
-  typed Γ e Tnat →
-  typed Γ (Output e) Tnat
+(* | typed_Input : *)
+(*   typed Γ Input Tnat *)
+(* | typed_Output e : *)
+(*   typed Γ e Tnat → *)
+(*   typed Γ (Output e) Tnat *)
 (* | typed_Throw e1 e2 τ τ' : *)
 (*   typed Γ e1 τ -> *)
 (*   typed Γ e2 (Tcont τ) -> *)
@@ -774,15 +885,15 @@ Global Instance IfNotationK {S : Set} {F G : Set -> Type} `{AsSynExpr F, AsSynEx
   }.
 
 
-Class OutputNotation (A B : Type) := { __output : A -> B }.
+(* Class OutputNotation (A B : Type) := { __output : A -> B }. *)
 
-Global Instance OutputNotationExpr {S : Set} {F : Set -> Type} `{AsSynExpr F} : OutputNotation (F S) (expr S) := {
-  __output e := Output (__asSynExpr e)
-  }.
+(* Global Instance OutputNotationExpr {S : Set} {F : Set -> Type} `{AsSynExpr F} : OutputNotation (F S) (expr S) := { *)
+(*   __output e := Output (__asSynExpr e) *)
+(*   }. *)
 
-Global Instance OutputNotationK {S : Set} : OutputNotation (ectx S) (ectx S) := {
-  __output K := K ++ [OutputK]
-  }.
+(* Global Instance OutputNotationK {S : Set} : OutputNotation (ectx S) (ectx S) := { *)
+(*   __output K := K ++ [OutputK] *)
+(*   }. *)
 
 Class ResetNotation (A B : Type) := { __reset : A -> B }.
 
@@ -827,10 +938,10 @@ Notation "x '+' y" := (__op x%syn Add y%syn) : syn_scope.
 Notation "x '-' y" := (__op x%syn Sub y%syn) : syn_scope.
 Notation "x '*' y" := (__op x%syn Mult y%syn) : syn_scope.
 Notation "'if' x 'then' y 'else' z" := (__if x%syn y%syn z%syn) : syn_scope.
-Notation "'output' x" := (__output x%syn) (at level 60) : syn_scope.
+(* Notation "'output' x" := (__output x%syn) (at level 60) : syn_scope. *)
 (* Notation "'throw' e₁ e₂" := (__throw e₁%syn e₂%syn) (at level 60) : syn_scope. *)
 Notation "'#' n" := (LitV n) (at level 60) : syn_scope.
-Notation "'input'" := (Input) : syn_scope.
+(* Notation "'input'" := (Input) : syn_scope. *)
 Notation "'rec' e" := (RecV e%syn) (at level 60) : syn_scope.
 Notation "'shift/cc' e" := (Shift e%syn) (at level 60) : syn_scope.
 Notation "'reset' e" := (Reset e%syn) (at level 60) : syn_scope.
@@ -895,34 +1006,34 @@ Module SynExamples.
 End SynExamples.
 
 Definition compute_head_step {S}
-  (e : expr S) (σ : state) (K : ectx S) :
-  option (expr S * state * ectx S * (nat * nat)) :=
+  (e : expr S) (K : ectx S) :
+  option (expr S * ectx S * (nat * nat)) :=
   match e with
   | (App (Val (RecV e1)) (Val v2)) =>
       Some ((subst (Inc := inc) ((subst (F := expr) (Inc := inc) e1)
                                    (Val (shift (Inc := inc) v2)))
-               (Val (RecV e1))), σ, K, (1,0))
-  | Input =>
-      let '(n, σ') := update_input σ in
-      Some ((Val (LitV n)), σ', K, (1, 1))
-  | Output (Val (LitV n)) =>
-      let σ' := update_output n σ in
-      Some ((Val (LitV 0)), σ', K, (1, 1))
+               (Val (RecV e1))), K, (1,0))
+  (* | Input => *)
+  (*     let '(n, σ') := update_input σ in *)
+  (*     Some ((Val (LitV n)), σ', K, (1, 1)) *)
+  (* | Output (Val (LitV n)) => *)
+  (*     (* let := update_output n σ in *) *)
+  (*     Some ((Val (LitV 0)), σ', K, (1, 1)) *)
   | (NatOp op (Val v1) (Val v2)) =>
       let res := nat_op_interp op v1 v2 in
-      option_rect (fun _ => option _) (fun v3 => Some ((Val v3), σ, K, (0, 0))) None res
+      option_rect (fun _ => option _) (fun v3 => Some ((Val v3), K, (0, 0))) None res
   | (If (Val (LitV n)) e1 e2) =>
       if (decide (0 < n))
-      then Some (e1, σ, K, (0, 0))
+      then Some (e1, K, (0, 0))
       else
         if (decide (n = 0))
-        then Some (e2, σ, K, (0, 0))
+        then Some (e2, K, (0, 0))
         else None
   (* | (Shift e) => *)
   (*     let (Ki, Ko) := shift_context K in *)
   (*     let f := cont_to_rec Ki in *)
-  (*     Some ((subst (Inc := inc) e (Val f)), σ, Ko, (1, 1)) *)
-  | (Reset (Val v)) => Some (Val v, σ, K, (1, 1))
+  (*     Some ((subst (Inc := inc) e (Val f)), Ko, (1, 1)) *)
+  | (Reset (Val v)) => Some (Val v, K, (1, 1))
   (* | (Reset (fill E (Shift e))) => None *)
   | _ => None
   end.
@@ -931,15 +1042,15 @@ Definition compute_head_step {S}
 Example test21 : val ∅ := (rec (if ($ 0) then # 1 else #0))%syn.
 
 
-Example testc : option (expr (inc ∅) * state * ectx (inc ∅) * (nat * nat)) :=
-  (compute_head_step (App (Val test1) (Val $ LitV 5)) (State [] []) []).
+Example testc : option (expr (inc ∅) * ectx (inc ∅) * (nat * nat)) :=
+  (compute_head_step (App (Val test1) (Val $ LitV 5)) []).
 Eval compute in testc.
 
 
-Lemma head_step_reflect {S : Set} (e : expr S) (σ : state) (K Ko : ectx S)
-  : option_reflect (fun '(e', σ', K', nm) => head_step e σ K e' σ' K' Ko nm)
+Lemma head_step_reflect {S : Set} (e : expr S) (K Ko : ectx S)
+  : option_reflect (fun '(e', K', nm) => head_step e K e' K' Ko nm)
       True
-      (compute_head_step e σ K).
+      (compute_head_step e  K).
 Proof.
   destruct e; try (by constructor).
   - destruct e1; try (by constructor).
@@ -971,14 +1082,14 @@ Proof.
         assumption.
       * constructor.
         constructor.
-  - simpl.
-    destruct (update_input σ) eqn:Heqn.
-    by do 2 constructor.
-  - simpl.
-    destruct e; try (by constructor).
-    destruct v; try (by constructor).
-    destruct (update_output n σ) eqn:Heqn.
-    by do 2 constructor.
+  (* - simpl. *)
+  (*   destruct (update_input σ) eqn:Heqn. *)
+  (*   by do 2 constructor. *)
+  (* - simpl. *)
+  (*   destruct e; try (by constructor). *)
+  (*   destruct v; try (by constructor). *)
+  (*   destruct (update_output n σ) eqn:Heqn. *)
+  (*   by do 2 constructor. *)
   (* - simpl. *)
   (*   destruct (shift_context K) as [Ki Ko] eqn:HK. *)
   (*   constructor. apply ShiftS with Ki =>//=. *)
